WIP

src/QUIC.Parse.fst
@@ -1,13 +1,10 @@
 module QUIC.Parse
 open QUIC.Spec.Base
+open QUIC.Parse.Lemmas
 
 open FStar.HyperStack.ST
 
 open LowParse.Spec.BitSum
-
-(* From
-https://tools.ietf.org/html/draft-ietf-quic-transport-23#section-16,
-except that we make the format non-ambiguous. *)
 
 open LowParse.Spec.BoundedInt
 
@@ -18,6 +15,230 @@ module U16 = FStar.UInt16
 module U8 = FStar.UInt8
 
 (* From https://tools.ietf.org/html/draft-ietf-quic-transport-23#section-17 *)
+
+(* BEGIN packet number *)
+
+(* From https://tools.ietf.org/html/draft-ietf-quic-transport-22#appendix-A *)
+
+inline_for_extraction
+noextract
+let integer_size = (x: nat { 1 <= x /\ x <= 4 })
+
+inline_for_extraction
+noextract
+let bounded_integer_prop
+  (sz: integer_size)
+  (x: U32.t)
+: Tot Type0
+= match sz with
+  | 1 -> U32.v x < 256
+  | 2 -> U32.v x < 65536
+  | 3 -> U32.v x < 16777216
+  | 4 -> True
+
+inline_for_extraction
+noextract
+let bounded_integer
+  (sz: integer_size)
+: Tot eqtype
+= (x: U32.t { bounded_integer_prop sz x })
+
+inline_for_extraction
+let bound_npn
+  (pn_len: packet_number_length_t)
+: Tot (x: U64.t { U64.v x == bound_npn' (U32.v pn_len - 1) })
+= if pn_len = 1ul
+  then 256uL
+  else if pn_len = 2ul
+  then 65536uL
+  else if pn_len = 3ul
+  then 16777216uL
+  else 4294967296uL
+
+let reduce_pn' pn_len pn = pn % (bound_npn' pn_len)
+
+inline_for_extraction
+let reduce_pn
+  (pn_len: packet_number_length_t)
+  (pn: uint62_t)
+: Tot (b: bounded_integer (U32.v pn_len) { U32.v b == reduce_pn' (U32.v pn_len - 1) (U64.v pn) })
+= [@inline_let]
+  let _ =
+    assert_norm (pow2 32 == 4294967296)
+  in
+  if pn_len = 4ul
+  then Cast.uint64_to_uint32 pn
+  else Cast.uint64_to_uint32 (pn `U64.rem` bound_npn pn_len)
+
+let in_window_self (pn_len: nat { pn_len < 4 }) (pn:nat) : Lemma
+  (in_window pn_len pn (if pn = 0 then 0 else pn - 1))
+= ()
+
+#push-options "--max_fuel 2 --initial_fuel 2 --max_ifuel 1 --initial_ifuel 1"
+let expand_pn'
+  (pn_len: nat { pn_len < 4 })
+  (last: nat { last + 1 < pow2 62})
+  (npn: nat { npn < bound_npn' pn_len })
+: Tot (pn: nat { pn < pow2 62 /\ in_window pn_len last pn /\ pn % bound_npn' pn_len == npn })
+=
+  let open FStar.Mul in
+  let open FStar.Math.Lemmas in
+  let expected = last + 1 in
+  let bound = bound_npn' pn_len in
+  let candidate = replace_modulo' expected bound npn in
+  lemma_replace_modulo_bound expected (8*(pn_len+1)) npn 62;
+  if candidate <= last + 1 - bound/2
+     && candidate < pow2 62 - bound then // the test for overflow (candidate < pow2 62 - bound) is not present in draft 22.
+    let _ = lemma_mod_plus candidate 1 bound in
+    candidate + bound
+  else if candidate > last + 1 + bound/2
+          && candidate >= bound then // in draft 22 the test for underflow (candidate >= bound) uses a strict inequality, which makes it impossible to expand npn to 0
+    let _ = lemma_mod_plus candidate (-1) bound in
+    candidate - bound
+  else candidate
+#pop-options
+
+let max (a b:int) : Tot (n:int{n >= a /\ n >= b}) =
+  if a > b then a else b // this must exist somewhere...
+
+let lemma_uniqueness_in_window (pn_len: nat { pn_len < 4 }) (last: nat { last < pow2 62 }) (x: nat {x < pow2 62}) (y:nat {y < pow2 62}) : Lemma
+  (requires (
+    let h = bound_npn' pn_len in
+    in_window pn_len last x /\
+    in_window pn_len last y /\
+    x%h = y%h))
+  (ensures x = y) =
+  let open FStar.Math.Lemmas in
+  pow2_lt_compat 62 (8 `op_Multiply` (pn_len+1));
+  let h = bound_npn' pn_len in
+  if last+1 < h/2 && x < h then
+    lemma_mod_plus_injective h 0 x y
+  else if last+1 >= pow2 62 - h/2 && x >= pow2 62 - h then
+    let low = pow2 62 - h in
+    lemma_mod_plus_injective h low (x-low) (y-low)
+  else
+    let low = max (last+2-h/2) 0 in
+    lemma_mod_plus_injective h low (x-low) (y-low)
+
+val lemma_parse_pn_correct : (pn_len: nat { pn_len < 4 }) -> last:nat{last+1 < pow2 62} -> (pn: nat { pn < U64.v uint62_bound }) -> Lemma
+  (requires in_window pn_len last pn)
+  (ensures expand_pn' pn_len last (reduce_pn' pn_len pn) = pn)
+
+let lemma_parse_pn_correct pn_len last pn =
+  lemma_uniqueness_in_window pn_len last pn (expand_pn' pn_len last (reduce_pn' pn_len pn))
+
+#push-options "--max_fuel 2 --initial_fuel 2 --max_ifuel 1 --initial_ifuel 1 --z3rlimit 64"
+
+let expand_pn
+  (pn_len: packet_number_length_t)
+  (last: last_packet_number_t)
+  (npn: bounded_integer (U32.v pn_len))
+: Tot (pn: uint62_t { U64.v pn == expand_pn' (U32.v pn_len - 1) (U64.v last) (U32.v npn) })
+= let open FStar.Mul in
+  let open FStar.Math.Lemmas in
+  let expected : uint62_t = last `U64.add` 1uL in
+  let bound = bound_npn pn_len in
+  let candidate = replace_modulo expected bound (Cast.uint32_to_uint64 npn) in
+  if (bound `U64.div` 2uL) `U64.lte` expected
+     && candidate `U64.lte` (expected `U64.sub` (bound `U64.div` 2uL))
+     && candidate `U64.lt` (uint62_bound `U64.sub` bound) then // the test for overflow (candidate < pow2 62 - bound) is not present in draft 22.
+//    let _ = lemma_mod_plus candidate 1 bound in
+    candidate `U64.add` bound
+  else if candidate `U64.gt` (expected `U64.add` (bound `U64.div` 2uL))
+          && candidate `U64.gte` bound then // in draft 22 the test for underflow (candidate >= bound) uses a strict inequality, which makes it impossible to expand npn to 0
+//    let _ = lemma_mod_plus candidate (-1) bound in
+    candidate `U64.sub` bound
+  else candidate
+#pop-options
+
+inline_for_extraction
+let packet_number_t
+  (last: last_packet_number_t)
+  (pn_len: packet_number_length_t)
+: Tot eqtype
+= (pn: uint62_t { in_window (U32.v pn_len - 1) (U64.v last) (U64.v pn) })
+
+inline_for_extraction
+let synth_packet_number
+  (last: last_packet_number_t)
+  (pn_len: packet_number_length_t)
+  (npn: bounded_integer (U32.v pn_len))
+: Tot (pn: packet_number_t last pn_len { U64.v pn == expand_pn' (U32.v pn_len - 1) (U64.v last) (U32.v npn) })
+= expand_pn pn_len last npn
+
+let parse_packet_number
+  (last: last_packet_number_t)
+  (pn_len: packet_number_length_t)
+: Tot (parser (parse_bounded_integer_kind (U32.v pn_len)) (packet_number_t last pn_len) )
+= parse_bounded_integer (U32.v pn_len) `parse_synth` synth_packet_number last pn_len
+
+inline_for_extraction
+let synth_packet_number_recip
+  (last: last_packet_number_t)
+  (pn_len: packet_number_length_t)
+  (pn: packet_number_t last pn_len)
+: Tot  (bounded_integer (U32.v pn_len))
+= reduce_pn pn_len pn
+
+let synth_packet_number_recip_inverse
+  (last: last_packet_number_t)
+  (pn_len: packet_number_length_t)
+: Lemma
+  (synth_inverse (synth_packet_number last pn_len) (synth_packet_number_recip last pn_len))
+//  [SMTPat (synth_inverse (synth_packet_number last pn_len) (synth_packet_number_recip last pn_len))] // TODO: WHY WHY WHY does this pattern not trigger?
+= synth_inverse_intro' #(bounded_integer (U32.v pn_len)) #(packet_number_t last pn_len) (synth_packet_number last pn_len) (synth_packet_number_recip last pn_len) (fun pn ->
+    lemma_parse_pn_correct (U32.v pn_len - 1) (U64.v last) (U64.v pn)
+  )
+
+let serialize_packet_number
+  (last: last_packet_number_t)
+  (pn_len: packet_number_length_t)
+: Tot (serializer (parse_packet_number last pn_len))
+= synth_packet_number_recip_inverse last pn_len;
+  serialize_synth
+    _
+    (synth_packet_number last pn_len)
+    (serialize_bounded_integer (U32.v pn_len))
+    (synth_packet_number_recip last pn_len)
+    ()
+
+#push-options "--z3rlimit 16"
+
+let serialize_packet_number_ext
+  (last1 last2: last_packet_number_t)
+  (pn_len: packet_number_length_t)
+  (pn: uint62_t)
+: Lemma
+  (requires (
+    in_window (U32.v pn_len - 1) (U64.v last1) (U64.v pn) /\
+    in_window (U32.v pn_len - 1) (U64.v last2) (U64.v pn)
+  ))
+  (ensures (
+    in_window (U32.v pn_len - 1) (U64.v last1) (U64.v pn) /\
+    in_window (U32.v pn_len - 1) (U64.v last2) (U64.v pn) /\
+    serialize (serialize_packet_number last1 pn_len) pn == serialize (serialize_packet_number last2 pn_len) pn
+  ))
+= synth_packet_number_recip_inverse last1 pn_len;
+  synth_packet_number_recip_inverse last2 pn_len;
+  serialize_synth_eq 
+    _
+    (synth_packet_number last1 pn_len)
+    (serialize_bounded_integer (U32.v pn_len))
+    (synth_packet_number_recip last1 pn_len)
+    ()
+    pn;
+  serialize_synth_eq 
+    _
+    (synth_packet_number last2 pn_len)
+    (serialize_bounded_integer (U32.v pn_len))
+    (synth_packet_number_recip last2 pn_len)
+    ()
+    pn
+
+#pop-options
+
+
+(* END packet number *)
 
 inline_for_extraction
 noextract
@@ -84,7 +305,7 @@ let rrpp : bitsum' uint8 4 =
 [@filter_bitsum'_t_attr]
 inline_for_extraction
 noextract
-let first_byte : bitsum' uint8 0 =
+let first_byte : bitsum' uint8 8 =
   BitSum' _ _ header_form (function
     | Short ->
       BitSum' _ _ fixed_bit (fun _ ->
@@ -117,9 +338,39 @@ let f (x: FStar.UInt8.t) : Tot unit =
   )
 *)
 
-open LowParse.Spec.Bytes
+inline_for_extraction
+let short_dcid_len_t = (short_dcid_len: U32.t { U32.v short_dcid_len <= 20 })
 
 module FB = FStar.Bytes
+
+let short_dcid_len_prop
+  (short_dcid_len: short_dcid_len_t)
+  (h: header)
+: GTot Type0
+= (MShort? h ==> dcid_len h == U32.v short_dcid_len)
+
+let packet_number_prop
+  (last: last_packet_number_t)
+  (h: header)
+: GTot Type0
+= ((~ (is_retry h)) ==> in_window (U32.v (pn_length h) - 1) (U64.v last) (U64.v (packet_number h)))
+
+unfold
+let parse_header_prop
+  (short_dcid_len: short_dcid_len_t)
+  (last: last_packet_number_t)
+  (m: header)
+: GTot Type0
+= short_dcid_len_prop short_dcid_len m /\
+  packet_number_prop last m
+
+inline_for_extraction
+type header'
+  (short_dcid_len: short_dcid_len_t)
+  (last: last_packet_number_t)
+= (m: header { parse_header_prop short_dcid_len last m })
+
+open LowParse.Spec.Bytes
 
 #push-options "--z3rlimit 16"
 
@@ -127,15 +378,15 @@ inline_for_extraction
 noextract
 let first_byte_of_header
   (short_dcid_len: short_dcid_len_t)
+  (last: last_packet_number_t)
   (t: Type0)
   (f: (bitsum'_type first_byte -> Tot t))
-  (m: header' short_dcid_len)
+  (m: header' short_dcid_len last)
 : Tot t
 = match m with
-  | MShort spin key_phase dcid packet_number ->
+  | MShort spin key_phase dcid pn_length packet_number ->
     let spin : bitfield uint8 1 = if spin then 1uy else 0uy in
     let key_phase : bitfield uint8 1 = if key_phase then 1uy else 0uy in
-    let pn_length : packet_number_length_t = FB.len packet_number in
     f (| Short, (| (), (spin, (| (), (key_phase, (| pn_length, () |) ) |) ) |) |)
   | MLong version dcid scid spec ->
     begin match spec with
@@ -162,9 +413,10 @@ let common_long_t
 inline_for_extraction
 noextract
 let payload_length_pn
+  (last: last_packet_number_t)
   (pn_length: packet_number_length_t)
 : Tot Type0
-= (varint_t & bounded_integer (U32.v pn_length))
+= (uint62_t & packet_number_t last pn_length)
 
 #push-options "--z3rlimit 16 --max_fuel 8 --max_ifuel 8 --initial_fuel 8 --initial_ifuel 8"
 
@@ -173,17 +425,18 @@ inline_for_extraction
 noextract
 let header_body_type
   (short_dcid_len: short_dcid_len_t)
+  (last: last_packet_number_t)
   (k' : bitsum'_key_type first_byte)
 : Tot Type0
 = match k' with
   | (| Short, (| (), (| (), (| pn_length, () |) |) |) |) ->
-    (FB.lbytes (U32.v short_dcid_len) & FB.lbytes (U32.v pn_length))
+    (FB.lbytes (U32.v short_dcid_len) & packet_number_t last pn_length)
   | (| Long, (| (), (| Initial, (| (), (| pn_length, () |) |) |) |) |) ->
-    (common_long_t & (parse_bounded_vlbytes_t 0 token_max_len & payload_length_pn pn_length))
+    (common_long_t & (parse_bounded_vlbytes_t 0 token_max_len & payload_length_pn last pn_length))
   | (| Long, (| (), (| ZeroRTT, (| (), (| pn_length, () |) |) |) |) |) ->
-    (common_long_t & payload_length_pn pn_length)
+    (common_long_t & payload_length_pn last pn_length)
   | (| Long, (| (), (| Handshake, (| (), (| pn_length, () |) |) |) |) |) ->
-    (common_long_t & payload_length_pn pn_length)
+    (common_long_t & payload_length_pn last pn_length)
   | (| Long, (| (), (| Retry, () |) |) |) ->
     (common_long_t & parse_bounded_vlbytes_t 0 20)
 
@@ -191,36 +444,37 @@ open LowParse.Spec.BitSum // again, for coerce
 
 #pop-options
 
-#push-options "--z3rlimit 32 --max_fuel 8 --max_ifuel 8 --initial_fuel 8 --initial_ifuel 8"
+#push-options "--z3rlimit 64 --max_fuel 8 --max_ifuel 8 --initial_fuel 8 --initial_ifuel 8"
 
 [@filter_bitsum'_t_attr]
 inline_for_extraction
 noextract
 let mk_header
   (short_dcid_len: short_dcid_len_t)
+  (last: last_packet_number_t)
   (k' : bitsum'_type first_byte)
-  (pl: header_body_type short_dcid_len (bitsum'_key_of_t first_byte k'))
-: Tot (refine_with_tag (first_byte_of_header short_dcid_len (bitsum'_type first_byte) id) k')
+  (pl: header_body_type short_dcid_len last (bitsum'_key_of_t first_byte k'))
+: Tot (refine_with_tag (first_byte_of_header short_dcid_len last (bitsum'_type first_byte) id) k')
 = match k' with
   | (| Short, (| (), (spin, (| (), (key_phase, (| pn_length, () |) ) |) ) |) |) ->
     let spin = (spin = 1uy) in
     let key_phase = (key_phase = 1uy) in
-    begin match coerce (FB.lbytes (U32.v short_dcid_len) & FB.lbytes (U32.v pn_length)) pl with
+    begin match coerce (FB.lbytes (U32.v short_dcid_len) & packet_number_t last pn_length) pl with
     | (dcid, packet_number) ->
-      MShort spin key_phase dcid packet_number
+      MShort spin key_phase dcid pn_length packet_number
     end
   | (| Long, (| (), (| Initial, (| (), (| pn_length, () |) |) |) |) |) ->
-    begin match coerce (common_long_t & (parse_bounded_vlbytes_t 0 token_max_len & payload_length_pn pn_length)) pl with
+    begin match coerce (common_long_t & (parse_bounded_vlbytes_t 0 token_max_len & payload_length_pn last pn_length)) pl with
     | ((version, (dcid, scid)), (token, (payload_length, packet_number))) ->
       MLong version dcid scid (MInitial token payload_length pn_length packet_number)
     end
   | (| Long, (| (), (| ZeroRTT, (| (), (| pn_length, () |) |) |) |) |) ->
-    begin match coerce (common_long_t & payload_length_pn pn_length) pl with
+    begin match coerce (common_long_t & payload_length_pn last pn_length) pl with
     | ((version, (dcid, scid)), (payload_length, packet_number)) ->
       MLong version dcid scid (MZeroRTT payload_length pn_length packet_number)
     end
   | (| Long, (| (), (| Handshake, (| (), (| pn_length, () |) |) |) |) |) ->
-    begin match coerce (common_long_t & payload_length_pn pn_length) pl with
+    begin match coerce (common_long_t & payload_length_pn last pn_length) pl with
     | ((version, (dcid, scid)), (payload_length, packet_number)) ->
       MLong version dcid scid (MHandshake payload_length pn_length packet_number)
     end
@@ -230,42 +484,39 @@ let mk_header
       MLong version dcid scid (MRetry unused odcid)
     end
 
-#pop-options
-
-#push-options "--z3rlimit 64 --max_fuel 8 --max_ifuel 8 --initial_fuel 8 --initial_ifuel 8"
-
 [@filter_bitsum'_t_attr]
 inline_for_extraction
 noextract
 let mk_header_body
   (short_dcid_len: short_dcid_len_t)
+  (last: last_packet_number_t)
   (k' : bitsum'_type first_byte)
-  (pl: refine_with_tag (first_byte_of_header short_dcid_len (bitsum'_type first_byte) id) k')
-: Tot (header_body_type short_dcid_len (bitsum'_key_of_t first_byte k'))
+  (pl: refine_with_tag (first_byte_of_header short_dcid_len last (bitsum'_type first_byte) id) k')
+: Tot (header_body_type short_dcid_len last (bitsum'_key_of_t first_byte k'))
 = match k' with
   | (| Short, (| (), (spin, (| (), (key_phase, (| pn_length, () |) ) |) ) |) |) ->
     begin match pl with
-    | MShort _ _ dcid pn -> coerce (header_body_type short_dcid_len (bitsum'_key_of_t first_byte k')) ((dcid, pn) <: (FB.lbytes (U32.v short_dcid_len) & FB.lbytes (U32.v pn_length)))
+    | MShort _ _ dcid _ pn -> coerce (header_body_type short_dcid_len last (bitsum'_key_of_t first_byte k')) ((dcid, pn) <: (FB.lbytes (U32.v short_dcid_len) & packet_number_t last pn_length ))
     end
   | (| Long, (| (), (| Initial, (| (), (| pn_length, () |) |) |) |) |) ->
     begin match pl with
     | MLong version dcid scid (MInitial token payload_length _ packet_number) ->
-      coerce (header_body_type short_dcid_len (bitsum'_key_of_t first_byte k')) (((version, (dcid, scid)), (token, (payload_length, packet_number))) <: (common_long_t & (parse_bounded_vlbytes_t 0 token_max_len & payload_length_pn pn_length)))
+      coerce (header_body_type short_dcid_len last (bitsum'_key_of_t first_byte k')) (((version, (dcid, scid)), (token, (payload_length, packet_number))) <: (common_long_t & (parse_bounded_vlbytes_t 0 token_max_len & payload_length_pn last pn_length)))
     end
   | (| Long, (| (), (| ZeroRTT, (| (), (| pn_length, () |) |) |) |) |) ->
     begin match pl with
     | MLong version dcid scid (MZeroRTT payload_length _ packet_number) ->
-      coerce (header_body_type short_dcid_len (bitsum'_key_of_t first_byte k')) (((version, (dcid, scid)), (payload_length, packet_number)) <: (common_long_t & payload_length_pn pn_length))
+      coerce (header_body_type short_dcid_len last (bitsum'_key_of_t first_byte k')) (((version, (dcid, scid)), (payload_length, packet_number)) <: (common_long_t & payload_length_pn last pn_length))
     end
   | (| Long, (| (), (| Handshake, (| (), (| pn_length, () |) |) |) |) |) ->
     begin match pl with
     | MLong version dcid scid (MHandshake payload_length _ packet_number) ->
-      coerce (header_body_type short_dcid_len (bitsum'_key_of_t first_byte k')) (((version, (dcid, scid)), (payload_length, packet_number)) <: (common_long_t & payload_length_pn pn_length))
+      coerce (header_body_type short_dcid_len last (bitsum'_key_of_t first_byte k')) (((version, (dcid, scid)), (payload_length, packet_number)) <: (common_long_t & payload_length_pn last pn_length))
     end
   | (| Long, (| (), (| Retry, (unused, ()) |) |) |) ->
     begin match pl with
     | MLong version dcid scid (MRetry unused odcid) ->
-      coerce (header_body_type short_dcid_len (bitsum'_key_of_t first_byte k')) (((version, (dcid, scid)), odcid) <: (common_long_t & parse_bounded_vlbytes_t 0 20))
+      coerce (header_body_type short_dcid_len last (bitsum'_key_of_t first_byte k')) (((version, (dcid, scid)), odcid) <: (common_long_t & parse_bounded_vlbytes_t 0 20))
     end
 
 [@filter_bitsum'_t_attr]
@@ -273,20 +524,21 @@ inline_for_extraction
 noextract
 let header_sum
   (short_dcid_len: short_dcid_len_t)
+  (last: last_packet_number_t)
 : Tot bitsum = BitSum
   _
   _
   _
   first_byte
   _
-  (first_byte_of_header short_dcid_len)
+  (first_byte_of_header short_dcid_len last)
   (fun _ _ _ -> ())
-  (header_body_type short_dcid_len)
+  (header_body_type short_dcid_len last)
   (SynthCase
-    #_ #_ #_ #first_byte #_ #(first_byte_of_header short_dcid_len) #(header_body_type short_dcid_len)
-    (mk_header short_dcid_len)
+    #_ #_ #_ #first_byte #_ #(first_byte_of_header short_dcid_len last) #(header_body_type short_dcid_len last)
+    (mk_header short_dcid_len last)
     (fun k x y -> ())
-    (mk_header_body short_dcid_len)
+    (mk_header_body short_dcid_len last)
     (fun k x -> ())
   )
 
@@ -295,29 +547,33 @@ let header_sum
 let parse_common_long : parser _ common_long_t =
   parse_flbytes 4 `nondep_then` (parse_bounded_vlbytes 0 20 `nondep_then` parse_bounded_vlbytes 0 20)
 
-let parse_payload_length_pn
-  (pn_length: packet_number_length_t)
-: Tot (parser _ (payload_length_pn pn_length))
-= parse_varint `nondep_then` parse_bounded_integer (U32.v pn_length)
+open QUIC.Parse.VarInt
 
-#push-options "--z3rlimit 32 --max_fuel 8 --max_ifuel 8 --initial_fuel 8 --initial_ifuel 8"
+let parse_payload_length_pn
+  (last: last_packet_number_t)
+  (pn_length: packet_number_length_t)
+: Tot (parser _ (payload_length_pn last pn_length))
+= parse_varint `nondep_then` parse_packet_number last pn_length
+
+#push-options "--z3rlimit 64 --max_fuel 8 --max_ifuel 8 --initial_fuel 8 --initial_ifuel 8"
 
 [@filter_bitsum'_t_attr]
 inline_for_extraction
 noextract
 let parse_header_body
   (short_dcid_len: short_dcid_len_t)
-  (k' : bitsum'_key_type (header_sum short_dcid_len).b)
-: Tot (k: parser_kind & parser k (bitsum_type_of_tag (header_sum short_dcid_len) k'))
+  (last: last_packet_number_t)
+  (k' : bitsum'_key_type (header_sum short_dcid_len last).b)
+: Tot (k: parser_kind & parser k (bitsum_type_of_tag (header_sum short_dcid_len last) k'))
 = match coerce (bitsum'_key_type first_byte) k' with
   | (| Short, (| (), (| (), (| pn_length, () |) |) |) |) ->
-    (| _, weaken (strong_parser_kind 0 20 None) (parse_flbytes (U32.v short_dcid_len)) `nondep_then` parse_flbytes (U32.v pn_length) |)
+    (| _, weaken (strong_parser_kind 0 20 None) (parse_flbytes (U32.v short_dcid_len)) `nondep_then` parse_packet_number last pn_length |)
   | (| Long, (| (), (| Initial, (| (), (| pn_length, () |) |) |) |) |) ->
-    (| _, parse_common_long `nondep_then` (parse_bounded_vlgenbytes 0 token_max_len (parse_bounded_varint 0 token_max_len) `nondep_then` parse_payload_length_pn pn_length) |)
+    (| _, parse_common_long `nondep_then` (parse_bounded_vlgenbytes 0 token_max_len (parse_bounded_varint 0 token_max_len) `nondep_then` parse_payload_length_pn last pn_length) |)
   | (| Long, (| (), (| ZeroRTT, (| (), (| pn_length, () |) |) |) |) |) ->
-    (| _, parse_common_long `nondep_then` parse_payload_length_pn pn_length |)
+    (| _, parse_common_long `nondep_then` parse_payload_length_pn last pn_length |)
   | (| Long, (| (), (| Handshake, (| (), (| pn_length, () |) |) |) |) |) ->
-    (| _, parse_common_long `nondep_then` parse_payload_length_pn pn_length |)
+    (| _, parse_common_long `nondep_then` parse_payload_length_pn last pn_length |)
   | (| Long, (| (), (| Retry, () |) |) |) ->
     (| _, parse_common_long `nondep_then` parse_bounded_vlbytes 0 20 |)
 
@@ -326,56 +582,61 @@ inline_for_extraction
 noextract
 let parse_header_kind'
   (short_dcid_len: short_dcid_len_t)
+  (last: last_packet_number_t)
 : Tot parser_kind
-= parse_bitsum_kind parse_u8_kind (header_sum short_dcid_len) (parse_header_body short_dcid_len)
+= parse_bitsum_kind parse_u8_kind (header_sum short_dcid_len last) (parse_header_body short_dcid_len last)
 
 inline_for_extraction
 noextract
 let parse_header_kind : parser_kind =
-  normalize_term (parse_header_kind' 0ul)
+  normalize_term (parse_header_kind' 0ul 0uL)
 
-let parse_header
+let lp_parse_header
   (short_dcid_len: short_dcid_len_t)
-: Tot (parser parse_header_kind (header' short_dcid_len))
-= assert_norm (parse_header_kind' short_dcid_len == parse_header_kind);
+  (last: last_packet_number_t)
+: Tot (parser parse_header_kind (header' short_dcid_len last))
+= assert_norm (parse_header_kind' short_dcid_len last == parse_header_kind);
   parse_bitsum
-    (header_sum short_dcid_len)
+    (header_sum short_dcid_len last)
     parse_u8
-    (parse_header_body short_dcid_len)
+    (parse_header_body short_dcid_len last)
 
 let serialize_common_long : serializer parse_common_long =
   serialize_flbytes 4 `serialize_nondep_then` (serialize_bounded_vlbytes 0 20 `serialize_nondep_then` serialize_bounded_vlbytes 0 20)
 
 let serialize_payload_length_pn
+  (last: last_packet_number_t)
   (pn_length: packet_number_length_t)
-: Tot (serializer (parse_payload_length_pn pn_length))
-= serialize_varint `serialize_nondep_then` serialize_bounded_integer (U32.v pn_length)
+: Tot (serializer (parse_payload_length_pn last pn_length))
+= serialize_varint `serialize_nondep_then` serialize_packet_number last pn_length
 
 let serialize_header_body
   (short_dcid_len: short_dcid_len_t)
-  (k' : bitsum'_key_type (header_sum short_dcid_len).b)
-: Tot (serializer (dsnd (parse_header_body short_dcid_len k')))
+  (last: last_packet_number_t)
+  (k' : bitsum'_key_type (header_sum short_dcid_len last).b)
+: Tot (serializer (dsnd (parse_header_body short_dcid_len last k')))
 = match coerce (bitsum'_key_type first_byte) k' with
   | (| Short, (| (), (| (), (| pn_length, () |) |) |) |) ->
-    serialize_weaken (strong_parser_kind 0 20 None) (serialize_flbytes (U32.v short_dcid_len)) `serialize_nondep_then` serialize_flbytes (U32.v pn_length)
+    serialize_weaken (strong_parser_kind 0 20 None) (serialize_flbytes (U32.v short_dcid_len)) `serialize_nondep_then` serialize_packet_number last pn_length
   | (| Long, (| (), (| Initial, (| (), (| pn_length, () |) |) |) |) |) ->
-    serialize_common_long `serialize_nondep_then` (serialize_bounded_vlgenbytes 0 token_max_len (serialize_bounded_varint 0 token_max_len) `serialize_nondep_then` serialize_payload_length_pn pn_length)
+    serialize_common_long `serialize_nondep_then` (serialize_bounded_vlgenbytes 0 token_max_len (serialize_bounded_varint 0 token_max_len) `serialize_nondep_then` serialize_payload_length_pn last pn_length)
   | (| Long, (| (), (| ZeroRTT, (| (), (| pn_length, () |) |) |) |) |) ->
-    serialize_common_long `serialize_nondep_then` serialize_payload_length_pn pn_length
+    serialize_common_long `serialize_nondep_then` serialize_payload_length_pn last pn_length
   | (| Long, (| (), (| Handshake, (| (), (| pn_length, () |) |) |) |) |) ->
-    serialize_common_long `serialize_nondep_then` serialize_payload_length_pn pn_length
+    serialize_common_long `serialize_nondep_then` serialize_payload_length_pn last pn_length
   | (| Long, (| (), (| Retry, () |) |) |) ->
     serialize_common_long `serialize_nondep_then` serialize_bounded_vlbytes 0 20
 
 let serialize_header
   (short_dcid_len: short_dcid_len_t)
-: Tot (serializer (parse_header short_dcid_len))
-= assert_norm (parse_header_kind' short_dcid_len == parse_header_kind);
+  (last: last_packet_number_t)
+: Tot (serializer (lp_parse_header short_dcid_len last))
+= assert_norm (parse_header_kind' short_dcid_len last == parse_header_kind);
   serialize_bitsum
-    (header_sum short_dcid_len)
+    (header_sum short_dcid_len last)
     serialize_u8
-    #(parse_header_body short_dcid_len)
-    (serialize_header_body short_dcid_len)
+    #(parse_header_body short_dcid_len last)
+    (serialize_header_body short_dcid_len last)
 
 module LC = LowParse.Low.Combinators
 module LB = LowParse.Low.Bytes
@@ -388,29 +649,40 @@ let validate_common_long : LC.validator parse_common_long =
   LB.validate_flbytes 4 4ul `LC.validate_nondep_then` (LB.validate_bounded_vlbytes 0 20 `LC.validate_nondep_then` LB.validate_bounded_vlbytes 0 20)
 
 inline_for_extraction
+let validate_packet_number
+  (last: last_packet_number_t)
+  (pn_len: packet_number_length_t)
+: Tot (LC.validator (parse_packet_number last pn_len))
+= LC.validate_synth
+    (LI.validate_bounded_integer (U32.v pn_len))
+    (synth_packet_number last pn_len)
+    ()
+
+inline_for_extraction
 noextract
 let validate_payload_length_pn
+  (last: last_packet_number_t)
   (pn_length: packet_number_length_t)
-: Tot (LC.validator (parse_payload_length_pn pn_length))
-= validate_varint `LC.validate_nondep_then` LI.validate_bounded_integer (U32.v pn_length)
-
+: Tot (LC.validator (parse_payload_length_pn last pn_length))
+= validate_varint `LC.validate_nondep_then` validate_packet_number last pn_length
 
 [@filter_bitsum'_t_attr]
 inline_for_extraction
 noextract
 let validate_header_body_cases
   (short_dcid_len: short_dcid_len_t)
-  (k' : bitsum'_key_type (header_sum short_dcid_len).b)
-: Tot (LC.validator (dsnd (parse_header_body short_dcid_len k')))
+  (last: last_packet_number_t)
+  (k' : bitsum'_key_type (header_sum short_dcid_len last).b)
+: Tot (LC.validator (dsnd (parse_header_body short_dcid_len last k')))
 = match coerce (bitsum'_key_type first_byte) k' with
   | (| Short, (| (), (| (), (| pn_length, () |) |) |) |) ->
-    LC.validate_weaken (strong_parser_kind 0 20 None) (LB.validate_flbytes (U32.v short_dcid_len) short_dcid_len) () `LC.validate_nondep_then` LB.validate_flbytes (U32.v pn_length) pn_length
+    LC.validate_weaken (strong_parser_kind 0 20 None) (LB.validate_flbytes (U32.v short_dcid_len) short_dcid_len) () `LC.validate_nondep_then` validate_packet_number last pn_length
   | (| Long, (| (), (| Initial, (| (), (| pn_length, () |) |) |) |) |) ->
-    validate_common_long `LC.validate_nondep_then` (LB.validate_bounded_vlgenbytes 0 0ul token_max_len (U32.uint_to_t token_max_len) (validate_bounded_varint 0ul (U32.uint_to_t token_max_len)) (read_bounded_varint 0 token_max_len) `LC.validate_nondep_then` validate_payload_length_pn pn_length)
+    validate_common_long `LC.validate_nondep_then` (LB.validate_bounded_vlgenbytes 0 0ul token_max_len (U32.uint_to_t token_max_len) (validate_bounded_varint 0ul (U32.uint_to_t token_max_len)) (read_bounded_varint 0 token_max_len) `LC.validate_nondep_then` validate_payload_length_pn last pn_length)
   | (| Long, (| (), (| ZeroRTT, (| (), (| pn_length, () |) |) |) |) |) ->
-    validate_common_long `LC.validate_nondep_then` validate_payload_length_pn pn_length
+    validate_common_long `LC.validate_nondep_then` validate_payload_length_pn last pn_length
   | (| Long, (| (), (| Handshake, (| (), (| pn_length, () |) |) |) |) |) ->
-    validate_common_long `LC.validate_nondep_then` validate_payload_length_pn pn_length
+    validate_common_long `LC.validate_nondep_then` validate_payload_length_pn last pn_length
   | (| Long, (| (), (| Retry, () |) |) |) ->
     validate_common_long `LC.validate_nondep_then` LB.validate_bounded_vlbytes 0 20
 
@@ -422,8 +694,9 @@ let filter_first_byte'
 inline_for_extraction
 let filter_first_byte
   (short_dcid_len: short_dcid_len_t)
-: Tot (filter_bitsum'_t (header_sum short_dcid_len).b)
-= coerce (filter_bitsum'_t (header_sum short_dcid_len).b) filter_first_byte'
+  (last: last_packet_number_t)
+: Tot (filter_bitsum'_t (header_sum short_dcid_len last).b)
+= coerce (filter_bitsum'_t (header_sum short_dcid_len last).b) filter_first_byte'
 
 inline_for_extraction
 noextract
@@ -436,21 +709,140 @@ inline_for_extraction
 noextract
 let mk_validate_header_body_cases
   (short_dcid_len: short_dcid_len_t)
-: LL.validate_bitsum_cases_t (header_sum short_dcid_len).b
-= coerce (LL.validate_bitsum_cases_t (header_sum short_dcid_len).b) mk_validate_header_body_cases' 
+  (last: last_packet_number_t)
+: LL.validate_bitsum_cases_t (header_sum short_dcid_len last).b
+= coerce (LL.validate_bitsum_cases_t (header_sum short_dcid_len last).b) mk_validate_header_body_cases' 
 
 let validate_header
   (short_dcid_len: short_dcid_len_t)
-: Tot (LL.validator (parse_header short_dcid_len))
-= assert_norm (parse_header_kind' short_dcid_len == parse_header_kind);
+  (last: last_packet_number_t)
+: Tot (LL.validator (lp_parse_header short_dcid_len last))
+= assert_norm (parse_header_kind' short_dcid_len last == parse_header_kind);
   LL.validate_bitsum
-    (header_sum short_dcid_len)
+    (header_sum short_dcid_len last)
     (LJ.validate_u8 ())
     LJ.read_u8
-    (filter_first_byte short_dcid_len)
-    (parse_header_body short_dcid_len)
-    (validate_header_body_cases short_dcid_len)
-    (mk_validate_header_body_cases short_dcid_len)
+    (filter_first_byte short_dcid_len last)
+    (parse_header_body short_dcid_len last)
+    (validate_header_body_cases short_dcid_len last)
+    (mk_validate_header_body_cases short_dcid_len last)
+
+#pop-options
+
+(* Properties of the serializer *)
+
+let serialize_header_ext
+  (cid_len1 cid_len2: short_dcid_len_t)
+  (last1 last2: last_packet_number_t)
+  (x: header)
+: Lemma
+  (requires (
+    parse_header_prop cid_len1 last1 x /\
+    parse_header_prop cid_len2 last2 x
+  ))
+  (ensures (
+    serialize (serialize_header cid_len1 last1) x == serialize (serialize_header cid_len2 last2) x
+  ))
+= admit ()
+
+(* Fulfill the interface *)
+
+let last_packet_number
+  (h: header)
+: Tot last_packet_number_t
+= if is_retry h then 0uL else let pn = packet_number h in if pn = 0uL then 0uL else pn `U64.sub` 1uL
+
+#push-options "--z3rlimit 32"
+
+let parse_header_prop_intro
+  (h: header)
+: Lemma
+  (parse_header_prop (U32.uint_to_t (dcid_len h)) (last_packet_number h) h)
+= ()
+
+#pop-options
+
+let format_header' (h: header) : GTot bytes =
+  parse_header_prop_intro h;
+  serialize (serialize_header (U32.uint_to_t (dcid_len h)) (last_packet_number h)) h
+
+let header_len h =
+  parse_header_prop_intro h;
+  Seq.length (format_header' h)
+
+let format_header h = format_header' h
+
+let format_header_is_short h =
+  assume (MShort? h <==> uint8.get_bitfield (Seq.index (format_header h) 0) 7 8 == (LowParse.Spec.Enum.enum_repr_of_key header_form Short <: U8.t))
+
+let format_header_is_retry h = admit ()
+
+let format_header_pn_length h = admit ()
+
+let pn_offset h = admit ()
+
+let putative_pn_offset cid_len x = admit ()
+
+let putative_pn_offset_frame cid_len x1 x2 = admit ()
+
+let putative_pn_offset_correct h cid_len = admit ()
+
+let parse_header cid_len last b =
+  match parse (lp_parse_header (U32.uint_to_t cid_len) (U64.uint_to_t last)) b with
+  | None -> H_Failure
+  | Some (h, consumed) -> H_Success h (Seq.slice b consumed (Seq.length b))
+
+module Seq = FStar.Seq
+
+#push-options "--z3rlimit 128"
+
+let lemma_header_parsing_correct
+  h c cid_len last
+=
+  parse_header_prop_intro h;
+  serialize_header_ext (U32.uint_to_t (dcid_len h)) (U32.uint_to_t cid_len) (last_packet_number h) (U64.uint_to_t last) h;
+  let s = format_header h in
+  assert (s == serialize (serialize_header (U32.uint_to_t cid_len) (U64.uint_to_t last)) h);
+  parse_serialize (serialize_header (U32.uint_to_t cid_len) (U64.uint_to_t last)) h;
+  parse_strong_prefix (lp_parse_header (U32.uint_to_t cid_len) (U64.uint_to_t last)) s (s `Seq.append` c);
+  match parse_header cid_len last Seq.(format_header h @| c) with
+  | H_Failure -> ()
+  | H_Success h' c' -> assert (h == h' /\ c `Seq.equal` c')
+
+#pop-options
+
+#push-options "--z3rlimit 64 --using_facts_from '*,-LowParse,+LowParse.Spec.Base'"
+
+let lemma_header_parsing_safe
+  cid_len last b1 b2
+= match parse_header cid_len last b1 with
+  | H_Failure -> ()
+  | H_Success h1 c1 ->
+    let consumed = Seq.length b1 - Seq.length c1 in
+    assert (Some? (parse (lp_parse_header (U32.uint_to_t cid_len) (U64.uint_to_t last)) b1)); //  == Some (h1, consumed));
+    let Some (h1', consumed') = parse (lp_parse_header (U32.uint_to_t cid_len) (U64.uint_to_t last)) b1 in
+    assert (h1 == h1');
+    let consumed' : consumed_length b1 = consumed' in
+    assert (consumed' <= Seq.length b1);
+    assert (c1 == Seq.slice b1 consumed' (Seq.length b1));
+    assert (consumed == consumed');
+    parse_injective (lp_parse_header (U32.uint_to_t cid_len) (U64.uint_to_t last)) b1 b2;
+    Seq.lemma_split b1 consumed;
+    assert (parse_header cid_len last b2 == H_Success h1 c1);
+    Seq.lemma_split b2 consumed;
+    assume (b1 == b2)
+
+#pop-options
+
+(*
+  match parse_header cid_len last b1, parse_header cid_len last b2 with
+  | H_Failure, _ -> ()
+  | H_Success h1 c1, H_Success h2 c2 -> assert (h1 == h2 /\ c1 `Seq.equal` c2); assume (b1 == b2)
+  | _ -> assert False
+*)
+
+(*
+let parse_header  cid_len b =
 
 let test b =
   let sl = LowParse.Slice.make_slice b 42ul in
