src/QUIC.Spec.Base.fst
@@ -7,13 +7,13 @@ module U8 = FStar.UInt8
 module S = FStar.Seq
 
 inline_for_extraction
-let varint_bound : (varint_bound: U64.t { U64.v varint_bound == pow2 62 }) =
+let uint62_bound : (uint62_bound: U64.t { U64.v uint62_bound == pow2 62 }) =
   [@inline_let] let v = 4611686018427387904uL in
   [@inline_let] let _ = assert_norm (U64.v v == pow2 62) in
   v
 
 inline_for_extraction
-let varint_t = (x: U64.t { U64.v x < U64.v varint_bound })
+let uint62_t = (x: U64.t { U64.v x < U64.v uint62_bound })
 
 type byte = FStar.UInt8.t
 type bytes = s:S.seq byte
@@ -22,29 +22,6 @@ type lbytes (n:nat) = b:bytes{S.length b = n}
 inline_for_extraction
 let vlbytes (min: nat) (max: nat) =
   (x: FB.bytes { min <= FB.length x /\ FB.length x <= max })
-
-inline_for_extraction
-noextract
-let integer_size = (x: nat { 1 <= x /\ x <= 4 })
-
-inline_for_extraction
-noextract
-let bounded_integer_prop
-  (sz: integer_size)
-  (x: U32.t)
-: Tot Type0
-= match sz with
-  | 1 -> U32.v x < 256
-  | 2 -> U32.v x < 65536
-  | 3 -> U32.v x < 16777296
-  | 4 -> True
-
-inline_for_extraction
-noextract
-let bounded_integer
-  (sz: integer_size)
-: Tot eqtype
-= (x: U32.t { bounded_integer_prop sz x })
 
 inline_for_extraction
 noextract
@@ -65,19 +42,19 @@ noeq
 type long_header_specifics =
 | MInitial:
   (token: vlbytes 0 token_max_len) -> // arbitrary bound
-  (payload_length: varint_t) ->
+  (payload_length: uint62_t) ->
   (packet_number_length: packet_number_length_t) ->
-  (packet_number: bounded_integer (U32.v packet_number_length)) ->
+  (packet_number: uint62_t) ->
   long_header_specifics
 | MZeroRTT:
-  (payload_length: varint_t) ->
+  (payload_length: uint62_t) ->
   (packet_number_length: packet_number_length_t) ->
-  (packet_number: bounded_integer (U32.v packet_number_length)) ->
+  (packet_number: uint62_t) ->
   long_header_specifics
 | MHandshake:
-  (payload_length: varint_t) ->
+  (payload_length: uint62_t) ->
   (packet_number_length: packet_number_length_t) ->
-  (packet_number: bounded_integer (U32.v packet_number_length)) ->
+  (packet_number: uint62_t) ->
   long_header_specifics
 | MRetry:
   (unused: bitfield 4) ->
@@ -95,9 +72,9 @@ type header =
 | MShort:
   (spin: bool) ->
   (key_phase: bool) ->
-  (dcid: FB.bytes) ->
+  (dcid: vlbytes 0 20) ->
   (packet_number_length: packet_number_length_t) ->
-  (packet_number: bounded_integer (U32.v packet_number_length)) ->
+  (packet_number: uint62_t) ->
   header
 
 let is_initial (h: header) : Tot bool =
@@ -122,7 +99,7 @@ let pn_length (h: header { ~ (is_retry h) }) : Tot packet_number_length_t =
     end
   | MShort _ _ _ pnl _ -> pnl
 
-let packet_number (h: header {~ (is_retry h)}) : Tot (bounded_integer (U32.v (pn_length h))) =
+let packet_number (h: header {~ (is_retry h)}) : Tot uint62_t =
   match h with
   | MLong _ _ _ spec ->
     begin match spec with
@@ -137,18 +114,7 @@ let dcid_len (h: header) : Tot nat =
   | MLong _ dcid _ _ -> FB.length dcid
   | MShort _ _ dcid _ _ -> FB.length dcid
 
-inline_for_extraction
-let short_dcid_len_t = (short_dcid_len: U32.t { U32.v short_dcid_len <= 20 })
-
-let header_short_dcid_length_prop
-  (m: header)
-  (short_dcid_len: short_dcid_len_t)
-: GTot bool
-= if MShort? m
-  then FB.length (MShort?.dcid m) = U32.v short_dcid_len
-  else true
-
-inline_for_extraction
-type header' (short_dcid_len: short_dcid_len_t) = (m: header { header_short_dcid_length_prop m short_dcid_len })
-
 type packet = b:bytes{let l = S.length b in 21 <= l /\ l < pow2 32}
+
+inline_for_extraction
+let last_packet_number_t = (last: uint62_t { U64.v last + 1 < U64.v uint62_bound})
