src/QUIC.Parse.Lemmas.fst
@@ -1,0 +1,58 @@
+module QUIC.Parse.Lemmas
+open QUIC.Spec.Base
+
+let replace_modulo' (a b new_mod:nat) : Pure nat
+  (requires b > 0 /\ new_mod < b)
+  (ensures fun res -> res % b = new_mod /\ res / b = a / b) =
+  let open FStar.Math.Lemmas in
+  let res = a - a%b + new_mod in
+  lemma_mod_plus new_mod (a/b) b;
+  small_mod new_mod b;
+  res
+
+#push-options "--z3rlimit 128"
+let lemma_replace_modulo_bound_aux (k:nat) (a:nat) (b:nat) (u:nat)
+  : Lemma (requires a < pow2 k /\ a % pow2 u == 0 /\ b < pow2 u /\ u < k)
+  (ensures a + b < pow2 k) =
+  let open FStar.Math.Lemmas in
+  let open FStar.Mul in
+  lemma_div_mod a (pow2 u);
+  assert(a + b == pow2 u * (a / pow2 u) + b);
+  lemma_div_plus b (a / pow2 u) (pow2 u);
+  small_div b (pow2 u);
+  lemma_div_lt_nat a k u;
+  assert((a / pow2 u) < pow2 (k-u));
+  assert(((a + b) / pow2 u) / pow2 (k-u) < 1);
+  division_multiplication_lemma (a+b) (pow2 u) (pow2 (k-u));
+  pow2_plus u (k-u)
+
+let lemma_replace_modulo_bound (a mod_pow new_mod up_pow:nat) : Lemma
+  (requires
+    mod_pow < up_pow /\
+    new_mod < pow2 mod_pow /\
+    a < pow2 up_pow)
+  (ensures replace_modulo' a (pow2 mod_pow) new_mod < pow2 up_pow) =
+  let open FStar.Math.Lemmas in
+  let open FStar.Mul in
+  let (pmod,umod) = (pow2 mod_pow, pow2 up_pow) in
+  lemma_div_mod a pmod;
+  multiple_modulo_lemma (a / pmod) pmod;
+  lemma_replace_modulo_bound_aux up_pow (a-a%pow2 mod_pow) new_mod mod_pow
+
+module U64 = FStar.UInt64
+
+#restart-solver
+
+inline_for_extraction
+let replace_modulo (a: uint62_t) (b new_mod: U64.t) : Pure U64.t
+  (requires U64.v b > 0 /\ U64.v new_mod < U64.v b)
+  (ensures fun res -> U64.v res == replace_modulo' (U64.v a) (U64.v b) (U64.v new_mod))
+=
+  let open FStar.Math.Lemmas in
+  [@inline_let] let _ =
+    lemma_mod_plus (U64.v new_mod) (U64.v a / U64.v b) (U64.v b);
+    small_mod (U64.v new_mod) (U64.v b)
+  in
+  (a `U64.sub` (a `U64.rem` b)) `U64.add` new_mod
+
+#pop-options
